wip monomorphiser

Test/Mono.lean
@@ -1,5 +1,26 @@
 import Nunchaku
 
+namespace Foo
+
+inductive MList (α : Type) where
+  | nil
+  | cons (x : α) (xs : MList α)
+
+def MList.map (xs : MList α) (f : α → β) : MList β :=
+  match xs with
+  | .nil => .nil
+  | .cons x xs => .cons (f x) (map xs f)
+
+set_option trace.nunchaku true in
+example  : MList.nil.map Nat.succ ≠ (.nil : MList Nat) := by
+  nunchaku
+
+end Foo
+
+set_option trace.nunchaku true in
+example  : [].map id ≠ ([] : List Nat) := by
+  nunchaku
+
 set_option trace.nunchaku true in
 example (xs : List α) : xs.map id ≠ xs := by
   nunchaku
@@ -12,7 +33,6 @@ set_option trace.nunchaku true in
 example (xs : List (List α)) : xs.map (·.map id) ≠ xs := by
   nunchaku
 
-
 def sumalt : List Nat → Nat :=
   List.foldr (· + ·) .zero
 
@@ -22,4 +42,12 @@ example (xs : List Nat) (h : xs ≠ []) : sumalt xs ≠ .zero := by
 
 set_option trace.nunchaku true in
 example (xs : List Nat) (h : xs ≠ []) : xs.sum ≠ .zero := by
+  nunchaku
+
+set_option trace.nunchaku true in
+example (xs : List (Fin n)) : xs.map id ≠ xs := by
+  nunchaku
+
+set_option trace.nunchaku true in
+example (xs : List (Fin .zero)) : ¬ xs.isEmpty := by
   nunchaku
